common/SmallstepLinkingSafe.v
@@ -29,58 +29,63 @@ Definition not_stuck {liA liB st} (L: lts liA liB st) (s: st) : Prop :=
 
 (* well-formed reachable state in module requires some restriction on
 incoming query and reply *)
-(* Inductive reachable {liA liB st} (IA: invariant liA) (IB: invariant liB) (L: lts liA liB st) (wI: inv_world IB) (s: st) : Prop := *)
-(* | initial_reach: forall q s0 t *)
-(*     (WT: query_inv IB wI q)     *)
-(*     (INIT: initial_state L q s0) *)
-(*     (STEP: Star L s0 t s), *)
-(*     reachable IA IB L wI s *)
-(* | external_reach: forall q r s1 s2 t w *)
-(*     (* s1 also must be reachable. TODO: s1 should be in at_external? *)
-(*     Otherwise we cannot prove reachable state is sound *)    *)
-(*     (REACH: reachable IA IB L wI s1) *)
-(*     (ATEXT: at_external L s1 q) *)
-(*     (WTQ: query_inv IA w q) *)
-(*     (WTR: reply_inv IA w r) *)
-(*     (AFEXT: after_external L s1 r s2) *)
-(*     (STEP: Star L s2 t s), *)
-(*     reachable IA IB L wI s. *)
+Inductive reachable {liA liB st} (IA: invariant liA) (IB: invariant liB) (L: lts liA liB st) (wI: inv_world IB) (s: st) : Prop :=
+| initial_reach: forall q s0 t
+    (WT: query_inv IB wI q)
+    (INIT: initial_state L q s0)
+    (STEP: Star L s0 t s),
+    reachable IA IB L wI s
+| external_reach: forall q r s1 s2 t w
+    (* s1 also must be reachable. TODO: s1 should be in at_external? *)
+(*     Otherwise we cannot prove reachable state is sound *)
+    (REACH: reachable IA IB L wI s1)
+    (ATEXT: at_external L s1 q)
+    (WTQ: query_inv IA w q)
+    (WTR: reply_inv IA w r)
+    (AFEXT: after_external L s1 r s2)
+    (STEP: Star L s2 t s),
+    reachable IA IB L wI s.
 
-(* Lemma reachable_implies liA liB st: forall IA IB (L: lts liA liB st) wI s, *)
-(*     reachable IA IB L wI s -> *)
-(*     SmallstepLinking.reachable L s. *)
-(* Proof. *)
-(*   induction 1. *)
-(*   try econstructor; eauto. *)
-(*   eapply SmallstepLinking.external_reach; eauto. *)
-(* Qed. *)
+Lemma step_reachable {liA liB st} IA IB (L: lts liA liB st) s1 t s2 w:
+  Step L s1 t s2 ->
+  reachable IA IB L w s1 ->
+  reachable IA IB L w s2.
+Proof.
+  intros STEP REA.
+  inv REA.
+  - eapply initial_reach; eauto.
+    eapply star_right; eauto.
+  - eapply external_reach; eauto.
+    eapply star_right; eauto.
+Qed.
 
-(* Record lts_safe {liA liB S} se (L: lts liA liB S) (IA: invariant liA) (IB: invariant liB) (SI: _ -> S -> Prop) (wI: inv_world IB) := *)
-(*   { *)
-(*     rechable_safe: forall s, *)
-(*       reachable IA IB L wI s -> *)
-(*       SI L s; *)
-    
-(*     (* compatable properties *) *)
-(*     initial_progress: forall q, *)
-(*       valid_query L q = true -> *)
-(*       query_inv IB wI q -> *)
-(*       (exists s, initial_state L q s); *)
-    
-(*     external_progress: forall s q, *)
-(*       reachable IA IB L wI s -> *)
-(*       at_external L s q -> *)
-(*       exists wA, symtbl_inv IA wA se /\ query_inv IA wA q /\ *)
-(*               forall r, reply_inv IA wA r -> *)
-(*                    (* after external progress *) *)
-(*                    (exists s', after_external L s r s'); *)
 
-(*     final_progress: forall s r, *)
-(*       reachable IA IB L wI s -> *)
-(*       final_state L s r -> *)
-(*       reply_inv IB wI r; *)
+Record lts_safe {liA liB S} se (L: lts liA liB S) (IA: invariant liA) (IB: invariant liB) (SI: _ -> S -> Prop) (wI: inv_world IB) :=
+  {
+    reachable_safe: forall s,
+      reachable IA IB L wI s ->
+      SI L s;
     
-(*   }. *)
+    (* properties of compositionality *)
+    initial_progress: forall q,
+      valid_query L q = true ->
+      query_inv IB wI q ->
+      (exists s, initial_state L q s);
+    
+    external_progress: forall s q,
+      reachable IA IB L wI s ->
+      at_external L s q ->
+      exists wA, symtbl_inv IA wA se /\ query_inv IA wA q /\
+              forall r, reply_inv IA wA r ->
+                   (* after external progress *)
+                   (exists s', after_external L s r s');
+
+    final_progress: forall s r,
+      reachable IA IB L wI s ->
+      final_state L s r ->
+      reply_inv IB wI r;
+    
+  }.
 
 (** Proof of lts_safe by the method of preservation and progress *)
 
@@ -96,124 +101,115 @@ incoming query and reply *)
       
       
 (*   } . *)
-    
-
-(** TODO: generalize safe/partial_safe to module linking and show that
-the original safe/partial_safe is identical to the composed
-safe/partial_safe *)
-
-(** TODO: essence behind the rechable predicate? i.e., how to prove
-lts_safe using lts_preserve in Invariant.v. TODO: try to define a
-proper rechable predicate to prove that lts_preserve /\ rechable ->
-sound_state *)
-Record lts_safe {liA liB S} se (L: lts liA liB S) (IA: invariant liA) (IB: invariant liB) (SI: _ -> S -> Prop) (wI: inv_world IB) :=
-  {
-    step_safe s t s' (REACH: reachable L s):
-    (* SI may be stronger than safe, but how to preserve the stronger part *)
-      (* SI L s -> *)
-      Step L s t s' ->
-      SI L s';
-    initial_safe q:
-      valid_query L q = true ->
-      query_inv IB wI q ->
-      (* initial_progress *)
-      (exists s, initial_state L q s)
-      (* initial_safe *)
-      /\ (forall s, initial_state L q s -> SI L s);
-    external_safe s q (REACH: reachable L s):
-      at_external L s q ->
-      exists wA, symtbl_inv IA wA se /\ query_inv IA wA q /\
-              forall r, reply_inv IA wA r ->
-                   (* after external progress *)
-                   (exists s', after_external L s r s')
-                   (* after external safe *)
-                   /\ (forall s', after_external L s r s' -> SI L s');
-    final_safe s r (REACH: reachable L s):
-      final_state L s r ->
-      reply_inv IB wI r;
-  }.
 
 
-(* se as an oracle, is it correct? *)
+(** Proof of compositionality of module safe *)
 Definition module_safe {liA liB} (L: semantics liA liB) (IA IB: invariant _) SI se :=
   forall w,
     Genv.valid_for (skel L) se ->
     symtbl_inv IB w se ->
     lts_safe se (L se) IA IB SI w.
 
+(* Propeties of reachable state in composed semantics *)
+Section REACH.
 
-Lemma safe_internal {li} (I: invariant li) L1 L2: forall i sk se s k w,
-    let L := fun (i:bool) => if i then L1 else L2 in
-    forall (Hsk: link (skel L1) (skel L2) = Some sk)
-      (VALID: Genv.valid_for (skel (SmallstepLinking.semantics L sk)) se)
-      (INV : symtbl_inv I w se)
-      (VALIDSE: forall i, Genv.valid_for (skel (L i)) se)
-      (SAFE: forall i, module_safe (L i) I I safe se)
-      (STSAFE: safe (L i se) s)
-      (WFSTATE: wf_state L se (st L i s :: k)),
-      safe (SmallstepLinking.semantics L sk se) (st L i s :: k).
+Context {li} (I: invariant li) (L: bool -> semantics li li). 
+Context (se: Genv.symtbl).
+Context (w: inv_world I).
+(* A generalized wf_state specifying rechable property and invariant world in the frame *)
+
+Inductive wf_frames : list (frame L) -> inv_world I -> Prop :=
+| wf_frames_nil: wf_frames nil w
+| wf_frames_cons: forall i s q w1 w2 fms
+    (WF: wf_frames fms w1)
+    (VSE1: symtbl_inv I w1 se)
+    (FREACH: reachable I I (L i se) w1 s)
+    (EXT: at_external (L i se) s q)
+    (WTQ: query_inv I w2 q)
+    (* (VSE2: symtbl_inv I w2 se) *)
+    (* desrible progress property here *)
+    (PGS: forall r, reply_inv I w2 r ->
+               exists s', after_external (L i se) s r s'),
+    wf_frames ((st L i s) :: fms) w2.
+
+Inductive wf_state : list (frame L) -> Prop :=
+| wf_state_cons: forall i s k w1
+    (WFS: wf_frames k w1)
+    (VSE: symtbl_inv I w1 se)
+    (SREACH: reachable I I (L i se) w1 s),
+    wf_state (st L i s :: k).
+
+
+Section SAFE.
+
+Hypothesis (VALIDSE: forall i, Genv.valid_for (skel (L i)) se).
+Hypothesis (SAFE: forall i, module_safe (L i) I I not_stuck se).
+
+Lemma step_wf_state sk s1 t s2:
+  Step (SmallstepLinking.semantics L sk se) s1 t s2 ->
+  wf_state s1 ->
+  wf_state s2.
 Proof.
-  intros.
-  destruct STSAFE as [(r & FINAL)|[(q & EXT)|(t1 & s1 & STEP1)]].
-  * destruct k.
-    -- left. exists r.
-       econstructor. auto.
-    -- destruct f.
-       right. right.
-       (* s0 in in at_external state *)
-       inv WFSTATE. subst_dep. inv H3. inv H2. subst_dep.
-       generalize (external_safe _ _ _ _ _ _ (SAFE i0 _ (VALIDSE i0) INV) s0 q H5 H3).
-       intros (wA & SYMBINV & QINV & AFTER).
-       generalize (final_safe _ _ _ _ _ _ (SAFE i _ (VALIDSE i) SYMBINV) _ _ H1 FINAL).
-       intros WR.
-       generalize (AFTER _ WR).
-       intros ((s0' & AFTER1) & SAFTER).
-       do 2 eexists.
-       eapply step_pop; eauto.
-  * inv WFSTATE. subst_dep.
-    generalize (external_safe _ _ _ _ _ _ (SAFE i _ (VALIDSE i) INV) s q H1 EXT).
+  intros STEP WF.
+  inv STEP.
+  - inv WF. subst_dep.
+    econstructor; eauto.
+    eapply step_reachable; eauto.
+  - inv WF. subst_dep.
+    (* external_progress of s *)    
+    exploit (@external_progress li); eauto. eapply SAFE; eauto.
     intros (wA & SYMBINV & QINV & AFTER).
-    destruct (valid_query (L i se) q) eqn: VQ1.
-    -- right. right.
-       generalize (initial_safe _ _ _ _ _ _ (SAFE i _ (VALIDSE i) SYMBINV) _ VQ1 QINV).
-       intros ((initS & INIT) & INITSAFE).
-       do 2 eexists.
-       eapply step_push; eauto.
-    -- destruct i; simpl in *.
-       ++ destruct (valid_query (L2 se) q) eqn: VQ2.
-          ** right. right.
-             generalize (initial_safe _ _ _ _ _ _ (SAFE false _ (VALIDSE false) SYMBINV) _ VQ2 QINV).
-             intros ((initS & INIT) & INITSAFE).
-             do 2 eexists.
-             eapply step_push. eauto.
-             instantiate (1 := false). auto.
-             simpl. eauto.
-          ** right. left.
-             eexists. econstructor.
-             simpl. eauto.
-             intros. destruct j; simpl; auto.
-       ++  destruct (valid_query (L1 se) q) eqn: VQ2.
-           ** right. right.
-              generalize (initial_safe _ _ _ _ _ _ (SAFE true _ (VALIDSE true) SYMBINV) _ VQ2 QINV).
-              intros ((initS & INIT) & INITSAFE).
-              do 2 eexists.
-              eapply step_push. eauto.
-              instantiate (1 := true). auto.
-              simpl. eauto.
-           ** right. left.
-              eexists. econstructor.
-              simpl. eauto.
-              intros. destruct j; simpl; auto.
-  * right. right. do 2 eexists.
-    eapply step_internal. simpl. eauto.
+    econstructor; eauto.
+    econstructor; eauto.
+    eapply initial_reach; eauto.
+    econstructor; eauto.
+  - inv WF. subst_dep.
+    exploit (@final_progress li); eauto. eapply SAFE; eauto.
+    intros WTR.
+    inv WFS. subst_dep.
+    econstructor; eauto.
+    eapply external_reach; eauto.
+    eapply star_refl.
+Qed.
+
+Lemma star_wf_state sk s1 t s2:
+  Star (SmallstepLinking.semantics L sk se) s1 t s2 ->
+  wf_state s1 ->
+  wf_state s2.
+Proof.
+  induction 1; auto.
+  intros WF. eapply IHstar.
+  eapply step_wf_state; eauto.
 Qed.
 
 
+Lemma reachable_wf_state sk s (WTSE: symtbl_inv I w se):
+  reachable I I (SmallstepLinking.semantics L sk se) w s ->
+  wf_state s.
+Proof.
+  induction 1.
+  - eapply star_wf_state; eauto.
+    inv INIT.
+    econstructor; eauto.
+    econstructor.
+    eapply initial_reach; eauto.
+    eapply star_refl.
+  - eapply star_wf_state; eauto.
+    inv AFEXT. inv ATEXT. inv IHreachable. subst_dep.
+    econstructor; eauto. 
+    eapply external_reach; eauto.
+    eapply star_refl.
+Qed.
+
+End SAFE.
+
+End REACH.
+
 Lemma compose_safety {li} (I: invariant li) L1 L2 L se:
-  module_safe L1 I I safe se ->
-  module_safe L2 I I safe se ->
+  module_safe L1 I I not_stuck se ->
+  module_safe L2 I I not_stuck se ->
   compose L1 L2 = Some L ->
-  module_safe L I I safe se.
+  module_safe L I I not_stuck se.
 Proof.
   intros SAFE1 SAFE2 COMP. unfold compose in *. unfold option_map in *.
   destruct (link (skel L1) (skel L2)) as [sk|] eqn:Hsk; try discriminate. inv COMP.
@@ -225,92 +221,307 @@ Proof.
   eapply (link_linkorder _ _ _ Hsk). eauto.
   eapply Genv.valid_for_linkorder.
   eapply (link_linkorder _ _ _ Hsk). eauto.
-  assert (SAFE: forall i, module_safe (L i) I I safe se).
+  assert (SAFE: forall i, module_safe (L i) I I not_stuck se).
   destruct i; simpl; auto.
   constructor.
-  - intros s t s' REACH STEP.
-    eapply reachable_wf_state in REACH.
-    inv STEP.
-    + (* destruct i; simpl in H. *)
-      assert (A: safe (L i se) s0). right. right. eauto.
-      assert (B: safe (L i se) s'0). {
-        eapply step_safe; eauto. eapply SAFE; eauto.
-        inv REACH. subst_dep. auto. }
-      eapply safe_internal; eauto.
-      inv REACH. subst_dep. econstructor;eauto. eapply step_reachable; eauto.
-    (* step_push *)
-    + assert (A: safe (L i se) s0). right. left. eauto.
-      assert (B: safe (L j se) s'0).
-      { inv REACH. subst_dep.
-        generalize (external_safe _ _ _ _ _ _ (SAFE i _ (VALIDSE i) INV) s0 q H4 H).
-        intros (wA & SYMBINV & QINV & AFTER).
-        eapply initial_safe. eapply SAFE; eauto. eauto. auto. auto. }
-      eapply safe_internal;eauto.
-      constructor; eauto. econstructor; eauto.
-      eapply star_refl.
-      inv REACH. subst_dep. econstructor;eauto.
-      econstructor;eauto.
-    (* step_pop *)
-    + inv REACH. inv H5. subst_dep.
-      inv H6. subst_dep.
-      assert (ATEXT: exists q, at_external (L j se) sk0 q).
-      eauto.
-      destruct ATEXT as (q1 & ATEXT).
-      generalize (external_safe _ _ _ _ _ _ (SAFE j _ (VALIDSE j) INV) sk0 q1 H5 ATEXT).
-      intros (wA & SYMBINV & QINV & AFTER).
-      generalize (final_safe _ _ _ _ _ _ (SAFE i _ (VALIDSE i) SYMBINV) _ _ H3 H).
-      intros VR.
-      generalize (AFTER r VR).
-      intros ((s' & AFTER1) & C).
-      assert (B: safe (L j se) s'0). eapply C. eauto.
-      eapply safe_internal; eauto.
-      econstructor;eauto. eapply external_reach. eapply H5. eapply H0.
-      eapply star_refl.
-  (* initial_safe *)
+  (* rechable not stuck *)
+  - intros s WFREACH.    
+    exploit (@reachable_wf_state li); eauto.
+    intros WFST.
+    (* destruct the frames to case analyze the top frame *)
+    destruct s. inv WFST.
+    destruct f. inv WFST. subst_dep.
+    (* s0 is not stuck because (L i) is safe *)
+    exploit (@reachable_safe li li (state (L i))); eauto.
+    eapply SAFE; eauto. intros SAFES0.
+    (* case analysis of not_stuck of s0 *)
+    destruct SAFES0 as [(r & FINAL)|[(q & EXT)|(t1 & s1 & STEP1)]].
+    (* s0 in final state *)
+    + destruct s.
+      (* composed semantics in final state *)
+      * red. left. exists r.
+        constructor. auto.
+      (* composed semantics can make a step to caller *)
+      * red. right. right.
+        inv WFS.
+        (* final_prgress in s0 *)
+        exploit (@final_progress li). eapply SAFE. eapply VALIDSE.
+        eapply VSE. eauto. eauto. intros WTR.        
+        exploit PGS; eauto. intros (s1' & AFEXT).
+        (* s0 can return a well-typed reply to s1 which is in at_external to make a step *)
+        do 2 eexists.
+        eapply step_pop; eauto.
+    (* s0 in at_external state *)
+    + exploit (@external_progress li); eauto.
+      eapply SAFE; eauto.
+      intros (wA & SYMBINV & QINV & AFTER). clear AFTER.
+      destruct (orb (valid_query (L true se) q) (valid_query (L false se) q)) eqn: VQ.
+      (* step_push *)
+      * eapply orb_true_iff in VQ.
+        red. right. right.
+        destruct VQ as [VQ1|VQ2].
+        -- exploit (@initial_progress li); eauto. eapply SAFE; eauto.
+           intros (s1 & INIT1).
+           do 2 eexists.        
+           eapply step_push; eauto. 
+        -- exploit (@initial_progress li); eauto. eapply SAFE; eauto.
+           intros (s1 & INIT1).
+           do 2 eexists.        
+           eapply step_push; eauto.
+      (* composed module in at_external *)
+      * red. right. left.
+        exists q. econstructor. eauto.
+        eapply orb_false_iff in VQ. destruct VQ.
+        intros. destruct j; auto.
+    (* s0 can make a step *)
+    + red. right. right.
+      do 2 eexists. eapply step_internal. eauto.
+  (* initial_progress *)
   - intros q VQ SQ. simpl in *.
     unfold SmallstepLinking.valid_query in VQ.
-    simpl in *. split.
-    + (* progress *)
-      destruct (valid_query (L1 se) q) eqn: VQ1.
-      * generalize (initial_safe _ _ _ _ _ _ (SAFE true _ (VALIDSE true) INV) _ VQ1 SQ).
-        intros ((s & INIT) & INITSAFE).
-        exists (st L true s :: nil). econstructor; eauto.
-      * rewrite orb_false_l in VQ.
-        generalize (initial_safe _ _ _ _ _ _ (SAFE false _ (VALIDSE false) INV) _ VQ SQ).
-        intros ((s & INIT) & INITSAFE).
-        exists (st L false s :: nil). econstructor; eauto.
-    + (* safe *)
-      intros s INIT.
-      inv INIT.
-      generalize (initial_safe _ _ _ _ _ _ (SAFE i _ (VALIDSE i) INV) _ H SQ).
-      intros ((s & INIT) & INITSAFE).
-      (* repeated work *)
-      clear INIT.
-      eapply safe_internal; eauto.
-      econstructor. eapply initial_reach; eauto.
-      eapply star_refl. constructor.  
+    eapply orb_true_iff in VQ. destruct VQ as [VQ1| VQ2].
+    + exploit (@initial_progress li); eauto.
+      eapply SAFE; eauto.
+      intros (s0 & INIT).
+      eexists. econstructor; eauto.
+    + exploit (@initial_progress li); eauto.
+      eapply SAFE; eauto.
+      intros (s0 & INIT).
+      eexists. econstructor; eauto.
+  (* external_progress *)
   - intros s q REACH EXT. inv EXT.
-    eapply reachable_wf_state in REACH. inv REACH. subst_dep.
-    generalize (external_safe _ _ _ _ _ _ (SAFE i _ (VALIDSE i) INV) s0 q H3 H).
+    eapply reachable_wf_state in REACH; eauto.
+    inv REACH. subst_dep.
+    exploit (@external_progress li); eauto. eapply SAFE; eauto.
     intros (wA & SYMBINV & QINV & AFTER).
     exists wA. split; auto. split; auto.
-    intros r SR.
-    generalize (AFTER r SR).
-    intros ((s' & AFTER1) & C).
-    split. exists (st L i s' :: k). econstructor; eauto.
-    intros s1' AFTER2. simpl in *. inv AFTER2. 
-    subst_dep.
-    generalize (C s'0 H8). intros D.
-    (* repeated work *)
-    eapply safe_internal; eauto.
-    econstructor; eauto. eapply external_reach; eauto.
-    eapply star_refl.    
+    intros r WTR.
+    exploit AFTER; eauto. intros (s1 & AFEXT).
+    exists (st L i s1 :: k).
+    constructor. auto.
+  (* final_progress *)
   - intros s r REACH FINAL.
     inv FINAL.
-    apply reachable_wf_state in REACH. inv REACH. subst_dep.
-    generalize (final_safe _ _ _ _ _ _ (SAFE i _ (VALIDSE i) INV) _ _ H2 H).
-    auto.
+    eapply reachable_wf_state in REACH; eauto. inv REACH. subst_dep.
+    inv WFS.
+    exploit (@final_progress li); eauto. eapply SAFE; eauto.
 Qed.
+
+
+(** Remove the following code (old lts_safe) *)
+(* (** TODO: generalize safe/partial_safe to module linking and show that *)
+(* the original safe/partial_safe is identical to the composed *)
+(* safe/partial_safe *) *)
+
+(* (** TODO: essence behind the rechable predicate? i.e., how to prove *)
+(* lts_safe using lts_preserve in Invariant.v. TODO: try to define a *)
+(* proper rechable predicate to prove that lts_preserve /\ rechable -> *)
+(* sound_state *) *)
+(* Record lts_safe {liA liB S} se (L: lts liA liB S) (IA: invariant liA) (IB: invariant liB) (SI: _ -> S -> Prop) (wI: inv_world IB) := *)
+(*   { *)
+(*     step_safe s t s' (REACH: reachable L s): *)
+(*     (* SI may be stronger than safe, but how to preserve the stronger part *) *)
+(*       (* SI L s -> *) *)
+(*       Step L s t s' -> *)
+(*       SI L s'; *)
+(*     initial_safe q: *)
+(*       valid_query L q = true -> *)
+(*       query_inv IB wI q -> *)
+(*       (* initial_progress *) *)
+(*       (exists s, initial_state L q s) *)
+(*       (* initial_safe *) *)
+(*       /\ (forall s, initial_state L q s -> SI L s); *)
+(*     external_safe s q (REACH: reachable L s): *)
+(*       at_external L s q -> *)
+(*       exists wA, symtbl_inv IA wA se /\ query_inv IA wA q /\ *)
+(*               forall r, reply_inv IA wA r -> *)
+(*                    (* after external progress *) *)
+(*                    (exists s', after_external L s r s') *)
+(*                    (* after external safe *) *)
+(*                    /\ (forall s', after_external L s r s' -> SI L s'); *)
+(*     final_safe s r (REACH: reachable L s): *)
+(*       final_state L s r -> *)
+(*       reply_inv IB wI r; *)
+(*   }. *)
+
+
+(* (* se as an oracle, is it correct? *) *)
+(* Definition module_safe {liA liB} (L: semantics liA liB) (IA IB: invariant _) SI se := *)
+(*   forall w, *)
+(*     Genv.valid_for (skel L) se -> *)
+(*     symtbl_inv IB w se -> *)
+(*     lts_safe se (L se) IA IB SI w. *)
+
+
+(* Lemma safe_internal {li} (I: invariant li) L1 L2: forall i sk se s k w, *)
+(*     let L := fun (i:bool) => if i then L1 else L2 in *)
+(*     forall (Hsk: link (skel L1) (skel L2) = Some sk) *)
+(*       (VALID: Genv.valid_for (skel (SmallstepLinking.semantics L sk)) se) *)
+(*       (INV : symtbl_inv I w se) *)
+(*       (VALIDSE: forall i, Genv.valid_for (skel (L i)) se) *)
+(*       (SAFE: forall i, module_safe (L i) I I safe se) *)
+(*       (STSAFE: safe (L i se) s) *)
+(*       (WFSTATE: wf_state L se (st L i s :: k)), *)
+(*       safe (SmallstepLinking.semantics L sk se) (st L i s :: k). *)
+(* Proof. *)
+(*   intros. *)
+(*   destruct STSAFE as [(r & FINAL)|[(q & EXT)|(t1 & s1 & STEP1)]]. *)
+(*   * destruct k. *)
+(*     -- left. exists r. *)
+(*        econstructor. auto. *)
+(*     -- destruct f. *)
+(*        right. right. *)
+(*        (* s0 in in at_external state *) *)
+(*        inv WFSTATE. subst_dep. inv H3. inv H2. subst_dep. *)
+(*        generalize (external_safe _ _ _ _ _ _ (SAFE i0 _ (VALIDSE i0) INV) s0 q H5 H3). *)
+(*        intros (wA & SYMBINV & QINV & AFTER). *)
+(*        generalize (final_safe _ _ _ _ _ _ (SAFE i _ (VALIDSE i) SYMBINV) _ _ H1 FINAL). *)
+(*        intros WR. *)
+(*        generalize (AFTER _ WR). *)
+(*        intros ((s0' & AFTER1) & SAFTER). *)
+(*        do 2 eexists. *)
+(*        eapply step_pop; eauto. *)
+(*   * inv WFSTATE. subst_dep. *)
+(*     generalize (external_safe _ _ _ _ _ _ (SAFE i _ (VALIDSE i) INV) s q H1 EXT). *)
+(*     intros (wA & SYMBINV & QINV & AFTER). *)
+(*     destruct (valid_query (L i se) q) eqn: VQ1. *)
+(*     -- right. right. *)
+(*        generalize (initial_safe _ _ _ _ _ _ (SAFE i _ (VALIDSE i) SYMBINV) _ VQ1 QINV). *)
+(*        intros ((initS & INIT) & INITSAFE). *)
+(*        do 2 eexists. *)
+(*        eapply step_push; eauto. *)
+(*     -- destruct i; simpl in *. *)
+(*        ++ destruct (valid_query (L2 se) q) eqn: VQ2. *)
+(*           ** right. right. *)
+(*              generalize (initial_safe _ _ _ _ _ _ (SAFE false _ (VALIDSE false) SYMBINV) _ VQ2 QINV). *)
+(*              intros ((initS & INIT) & INITSAFE). *)
+(*              do 2 eexists. *)
+(*              eapply step_push. eauto. *)
+(*              instantiate (1 := false). auto. *)
+(*              simpl. eauto. *)
+(*           ** right. left. *)
+(*              eexists. econstructor. *)
+(*              simpl. eauto. *)
+(*              intros. destruct j; simpl; auto. *)
+(*        ++  destruct (valid_query (L1 se) q) eqn: VQ2. *)
+(*            ** right. right. *)
+(*               generalize (initial_safe _ _ _ _ _ _ (SAFE true _ (VALIDSE true) SYMBINV) _ VQ2 QINV). *)
+(*               intros ((initS & INIT) & INITSAFE). *)
+(*               do 2 eexists. *)
+(*               eapply step_push. eauto. *)
+(*               instantiate (1 := true). auto. *)
+(*               simpl. eauto. *)
+(*            ** right. left. *)
+(*               eexists. econstructor. *)
+(*               simpl. eauto. *)
+(*               intros. destruct j; simpl; auto. *)
+(*   * right. right. do 2 eexists. *)
+(*     eapply step_internal. simpl. eauto. *)
+(* Qed. *)
+
+
+(* Lemma compose_safety {li} (I: invariant li) L1 L2 L se: *)
+(*   module_safe L1 I I safe se -> *)
+(*   module_safe L2 I I safe se -> *)
+(*   compose L1 L2 = Some L -> *)
+(*   module_safe L I I safe se. *)
+(* Proof. *)
+(*   intros SAFE1 SAFE2 COMP. unfold compose in *. unfold option_map in *. *)
+(*   destruct (link (skel L1) (skel L2)) as [sk|] eqn:Hsk; try discriminate. inv COMP. *)
+(*   set (L := fun i:bool => if i then L1 else L2). *)
+(*   red. intros w VALID INV. *)
+(*   assert (VALIDSE: forall i, Genv.valid_for (skel (L i)) se). *)
+(*   destruct i. *)
+(*   eapply Genv.valid_for_linkorder. *)
+(*   eapply (link_linkorder _ _ _ Hsk). eauto. *)
+(*   eapply Genv.valid_for_linkorder. *)
+(*   eapply (link_linkorder _ _ _ Hsk). eauto. *)
+(*   assert (SAFE: forall i, module_safe (L i) I I safe se). *)
+(*   destruct i; simpl; auto. *)
+(*   constructor. *)
+(*   - intros s t s' REACH STEP. *)
+(*     eapply reachable_wf_state in REACH. *)
+(*     inv STEP. *)
+(*     + (* destruct i; simpl in H. *) *)
+(*       assert (A: safe (L i se) s0). right. right. eauto. *)
+(*       assert (B: safe (L i se) s'0). { *)
+(*         eapply step_safe; eauto. eapply SAFE; eauto. *)
+(*         inv REACH. subst_dep. auto. } *)
+(*       eapply safe_internal; eauto. *)
+(*       inv REACH. subst_dep. econstructor;eauto. eapply step_reachable; eauto. *)
+(*     (* step_push *) *)
+(*     + assert (A: safe (L i se) s0). right. left. eauto. *)
+(*       assert (B: safe (L j se) s'0). *)
+(*       { inv REACH. subst_dep. *)
+(*         generalize (external_safe _ _ _ _ _ _ (SAFE i _ (VALIDSE i) INV) s0 q H4 H). *)
+(*         intros (wA & SYMBINV & QINV & AFTER). *)
+(*         eapply initial_safe. eapply SAFE; eauto. eauto. auto. auto. } *)
+(*       eapply safe_internal;eauto. *)
+(*       constructor; eauto. econstructor; eauto. *)
+(*       eapply star_refl. *)
+(*       inv REACH. subst_dep. econstructor;eauto. *)
+(*       econstructor;eauto. *)
+(*     (* step_pop *) *)
+(*     + inv REACH. inv H5. subst_dep. *)
+(*       inv H6. subst_dep. *)
+(*       assert (ATEXT: exists q, at_external (L j se) sk0 q). *)
+(*       eauto. *)
+(*       destruct ATEXT as (q1 & ATEXT). *)
+(*       generalize (external_safe _ _ _ _ _ _ (SAFE j _ (VALIDSE j) INV) sk0 q1 H5 ATEXT). *)
+(*       intros (wA & SYMBINV & QINV & AFTER). *)
+(*       generalize (final_safe _ _ _ _ _ _ (SAFE i _ (VALIDSE i) SYMBINV) _ _ H3 H). *)
+(*       intros VR. *)
+(*       generalize (AFTER r VR). *)
+(*       intros ((s' & AFTER1) & C). *)
+(*       assert (B: safe (L j se) s'0). eapply C. eauto. *)
+(*       eapply safe_internal; eauto. *)
+(*       econstructor;eauto. eapply external_reach. eapply H5. eapply H0. *)
+(*       eapply star_refl. *)
+(*   (* initial_safe *) *)
+(*   - intros q VQ SQ. simpl in *. *)
+(*     unfold SmallstepLinking.valid_query in VQ. *)
+(*     simpl in *. split. *)
+(*     + (* progress *) *)
+(*       destruct (valid_query (L1 se) q) eqn: VQ1. *)
+(*       * generalize (initial_safe _ _ _ _ _ _ (SAFE true _ (VALIDSE true) INV) _ VQ1 SQ). *)
+(*         intros ((s & INIT) & INITSAFE). *)
+(*         exists (st L true s :: nil). econstructor; eauto. *)
+(*       * rewrite orb_false_l in VQ. *)
+(*         generalize (initial_safe _ _ _ _ _ _ (SAFE false _ (VALIDSE false) INV) _ VQ SQ). *)
+(*         intros ((s & INIT) & INITSAFE). *)
+(*         exists (st L false s :: nil). econstructor; eauto. *)
+(*     + (* safe *) *)
+(*       intros s INIT. *)
+(*       inv INIT. *)
+(*       generalize (initial_safe _ _ _ _ _ _ (SAFE i _ (VALIDSE i) INV) _ H SQ). *)
+(*       intros ((s & INIT) & INITSAFE). *)
+(*       (* repeated work *) *)
+(*       clear INIT. *)
+(*       eapply safe_internal; eauto. *)
+(*       econstructor. eapply initial_reach; eauto. *)
+(*       eapply star_refl. constructor.   *)
+(*   - intros s q REACH EXT. inv EXT. *)
+(*     eapply reachable_wf_state in REACH. inv REACH. subst_dep. *)
+(*     generalize (external_safe _ _ _ _ _ _ (SAFE i _ (VALIDSE i) INV) s0 q H3 H). *)
+(*     intros (wA & SYMBINV & QINV & AFTER). *)
+(*     exists wA. split; auto. split; auto. *)
+(*     intros r SR. *)
+(*     generalize (AFTER r SR). *)
+(*     intros ((s' & AFTER1) & C). *)
+(*     split. exists (st L i s' :: k). econstructor; eauto. *)
+(*     intros s1' AFTER2. simpl in *. inv AFTER2.  *)
+(*     subst_dep. *)
+(*     generalize (C s'0 H8). intros D. *)
+(*     (* repeated work *) *)
+(*     eapply safe_internal; eauto. *)
+(*     econstructor; eauto. eapply external_reach; eauto. *)
+(*     eapply star_refl.     *)
+(*   - intros s r REACH FINAL. *)
+(*     inv FINAL. *)
+(*     apply reachable_wf_state in REACH. inv REACH. subst_dep. *)
+(*     generalize (final_safe _ _ _ _ _ _ (SAFE i _ (VALIDSE i) INV) _ _ H2 H). *)
+(*     auto. *)
+(* Qed. *)
 
 
 (* similar to ccref *)
